{
    "@graph": [
        {
            "@id": "adex:Text",
            "@type": [
                "rdfs:Class"
            ],
            "rdfs:comment": "Data type: Text for string values",
            "rdfs:label": "Text",
            "skos:exactMatch": {
                "@id": "schema:Text"
            }
        },
        {
            "@id": "adex:dataQualityFile",
            "@type": [
                "adex:Relationship"
            ],
            "rdfs:comment": " Data Quality file download link for the resource",
            "rdfs:label": "dataQualityFile",
            "adex:domainIncludes": [
                {
                    "@id": "adex:ResourceGroup"
                },
                {
                    "@id": "adex:Resource"
                }
            ],
            "adex:rangeIncludes": [
                {
                    "@container": "@list",
                    "@id": "adex:Text"
                },
                {
                    "@container": "@list",
                    "@id": "adex:RelationshipValue"
                }
            ],
            "rdfs:isDefinedBy": {
                "@id": "adex:"
            }
        },
        {
            "@id": "adex:address",
            "@type": [
                "adex:GeoProperty"
            ],
            "rdfs:comment": "Physical address of a place.",
            "rdfs:label": "address",
            "adex:domainIncludes": [
                {
                    "@id": "adex:Place"
                }
            ],
            "adex:rangeIncludes": [
                {
                    "@id": "adex:Text"
                },
                {
                    "@id": "adex:ValueDescriptor"
                }
            ],
            "rdfs:isDefinedBy": {
                "@id": "adex:"
            },
            "skos:exactMatch": {
                "@id": "schema:address"
            }
        },
        {
            "@id": "adex:resourceServerFileAccessURL",
            "@type": [
                "adex:Relationship"
            ],
            "rdfs:comment": "Resource Server URL for file access",
            "rdfs:label": "resourceServerFileAccessURL",
            "adex:domainIncludes": [
                {
                    "@id": "adex:ResourceServer"
                }
            ],
            "adex:rangeIncludes": [
                {
                    "@id": "adex:Text",
                    "@type": "@id"
                }
            ]
        },
        {
            "@id": "adex:sameAs",
            "@type": [
                "adex:TextProperty"
            ],
            "rdfs:comment": "URL reference to another thing/entity that identifies the given thing/entity. This may be used to provide references to another data models where a property is described or say a reference to Wiki pages for a given thing etc.",
            "rdfs:label": "sameAs",
            "adex:domainIncludes": [
                {
                    "@id": "adex:ValueDescriptor"
                }
            ],
            "adex:rangeIncludes": [
                {
                    "@id": "adex:Text",
                    "@type": "@id"
                }
            ],
            "skos:exactMatch": {
                "@id": "schema:sameAs"
            },
            "rdfs:isDefinedBy": {
                "@id": "adex:"
            }
        },
        {
            "@id": "adex:resourceServerHTTPAccessURL",
            "@type": [
                "adex:Relationship"
            ],
            "rdfs:comment": "Resource Server URL for data access based on HTTP/REST APIs",
            "rdfs:label": "resourceServerHTTPAccessURL",
            "adex:domainIncludes": [
                {
                    "@id": "adex:ResourceServer"
                }
            ],
            "adex:rangeIncludes": [
                {
                    "@id": "adex:Text",
                    "@type": "@id"
                }
            ]
        },
        {
            "@id": "adex:date",
            "@type": [
                "adex:TextProperty"
            ],
            "rdfs:comment": "Date corresponding to this observation and is described in YYYY-MM-DD format, for eg. '2020-11-01'.",
            "rdfs:label": "date",
            "adex:domainIncludes": [],
            "adex:rangeIncludes": [
                {
                    "@id": "adex:Text"
                },
                {
                    "@id": "adex:ValueDescriptor"
                }
            ],
            "rdfs:isDefinedBy": {
                "@id": "adex:"
            }
        },
        {
            "@id": "adex:resourceGroup",
            "@type": [
                "adex:Relationship"
            ],
            "rdfs:comment": "IRI pointing to the resourceGroup entity associated with the resource.",
            "rdfs:label": "resourceGroup",
            "adex:domainIncludes": [
                {
                    "@id": "adex:Resource",
                    "adex:requiredProperty": true
                }
            ],
            "adex:rangeIncludes": [
                {
                    "@id": "adex:Text",
                    "@type": "@id"
                },
                {
                    "@id": "adex:RelationshipValue"
                }
            ]
        },
        {
            "@id": "adex:accessObject",
            "@type": [
                "adex:Relationship"
            ],
            "rdfs:comment": "Link to the access object. For example, an open API object.",
            "rdfs:label": "accessObject",
            "adex:domainIncludes": [
                {
                    "@id": "adex:AccessObjectInfoValue"
                }
            ],
            "adex:rangeIncludes": [
                {
                    "@id": "adex:Text",
                    "@type": "@id"
                },
                {
                    "@id": "adex:RelationshipValue"
                }
            ]
        },
        {
            "@id": "adex:additionalInfoURL",
            "@type": [
                "adex:Relationship"
            ],
            "rdfs:comment": "URL from which additional information of the subject can be obtained",
            "rdfs:label": "additionalInfoURL",
            "adex:domainIncludes": [
                {
                    "@id": "adex:AccessObjectInfoValue"
                },
                {
                    "@id": "adex:Organization"
                }
            ],
            "adex:rangeIncludes": [
                {
                    "@id": "adex:Text",
                    "@type": "@id"
                },
                {
                    "@id": "adex:RelationshipValue"
                }
            ]
        },
        {
            "@id": "adex:relationType",
            "@type": [
                "adex:TextProperty"
            ],
            "rdfs:comment": "Type of relation. ENUM: [REL_MESSAGESTREAM, REL_FILE, REL_DATASET, REL_THING].",
            "rdfs:label": "relationType",
            "adex:domainIncludes": [
                {
                    "@id": "adex:RelationshipValue",
                    "adex:requiredProperty": true
                }
            ],
            "adex:rangeIncludes": [
                {
                    "@id": "adex:Text"
                },
                {
                    "@id": "adex:ValueDescriptor"
                }
            ],
            "rdfs:isDefinedBy": {
                "@id": "adex:"
            }
        },
        {
            "@id": "adex:provider",
            "@type": [
                "adex:Relationship"
            ],
            "rdfs:comment": "IRI pointing to the provider entity associated with the given catalogue item",
            "rdfs:label": "provider",
            "adex:domainIncludes": [
                {
                    "@id": "adex:Resource"
                },
                {
                    "@id": "adex:ResourceGroup",
                    "adex:requiredProperty": true
                }
            ],
            "adex:rangeIncludes": [
                {
                    "@id": "adex:Text",
                    "@type": "@id"
                },
                {
                    "@id": "adex:RelationshipValue"
                }
            ]
        },
        {
            "@id": "adex:dataDescriptor",
            "@type": [
                "adex:Relationship"
            ],
            "rdfs:comment": "URI pointing to the data-descriptor entity",
            "rdfs:label": "dataDescriptor",
            "adex:domainIncludes": [
                {
                    "@id": "adex:ResourceGroup"
                },
                {
                    "@id": "adex:Resource"
                }
            ],
            "adex:rangeIncludes": [
                {
                    "@type": "@id",
                    "@id": "adex:Text"
                },
                {
                    "@id": "adex:RelationshipValue"
                },
                {
                    "@id": "adex:DataModel"
                }
            ]
        },
        {
            "@id": "adex:description",
            "@type": [
                "adex:TextProperty"
            ],
            "rdfs:comment": "Description for an ADEX thing.",
            "rdfs:label": "description",
            "adex:domainIncludes": [
                {
                    "@id": "adex:Thing"
                }
            ],
            "adex:rangeIncludes": [
                {
                    "@id": "adex:Text"
                }
            ],
            "rdfs:isDefinedBy": {
                "@id": "adex:"
            }
        },
        {
            "@id": "adex:unitText",
            "@type": [
                "adex:TextProperty"
            ],
            "rdfs:comment": "Describes the unit of measurement. Useful if unitCode is not available.",
            "rdfs:label": "unitText",
            "adex:domainIncludes": [
                {
                    "@id": "adex:ValueDescriptor"
                }
            ],
            "adex:rangeIncludes": [
                {
                    "@id": "adex:Text"
                }
            ],
            "skos:exactMatch": {
                "@id": "schema:unitText"
            },
            "rdfs:isDefinedBy": {
                "@id": "adex:"
            }
        },
        {
            "@id": "adex:downloadURL",
            "@type": [
                "adex:Relationship"
            ],
            "rdfs:comment": "A download URL specifying the protocol, for e.g s3:// or https://, etc.",
            "rdfs:label": "downloadURL",
            "rdfs:isDefinedBy": {
                "@id": "adex:"
            },
            "adex:domainIncludes": [],
            "adex:rangeIncludes": [
                {
                    "@id": "adex:Text",
                    "@type": "@id"
                },
                {
                    "@id": "adex:RelationshipValue"
                }
            ]
        },
        {
            "@id": "adex:manufacturerName",
            "@type": [
                "adex:TextProperty"
            ],
            "rdfs:comment": "Name of the manufacturer associated with an entity, e.g., sensor, device etc.",
            "rdfs:label": "manufacturerName",
            "rdfs:isDefinedBy": {
                "@id": "adex:"
            },
            "adex:domainIncludes": [
                {
                    "@id": "adex:ModelInfo"
                }
            ],
            "adex:rangeIncludes": [
                {
                    "@id": "adex:Text"
                }
            ],
            "skos:exactMatch": {
                "@id": "Fiware:manufacturerName"
            }
        },
        {
            "@id": "adex:tags",
            "@type": [
                "adex:TextProperty"
            ],
            "rdfs:comment": "Comma separated discovery tags associated with an ADEXEntity (resource , resource Group)",
            "rdfs:label": "tags",
            "adex:domainIncludes": [
                {
                    "@id": "adex:Resource",
                    "adex:requiredProperty": true
                },
                {
                    "@id": "adex:ResourceGroup",
                    "adex:requiredProperty": true
                }
            ],
            "adex:rangeIncludes": [
                {
                    "@container": "@list",
                    "@id": "adex:Text"
                }
            ]
        },
        {
            "@id": "adex:associatedEntity",
            "@type": [
                "adex:Relationship"
            ],
            "rdfs:comment": "ID of the associated entity.",
            "rdfs:label": "associatedEntity",
            "adex:domainIncludes": [
                {
                    "@id": "adex:ADEXEntity"
                }
            ],
            "adex:rangeIncludes": [
                {
                    "@id": "adex:Text"
                },
                {
                    "@id": "adex:RelationshipValue"
                }
            ],
            "rdfs:isDefinedBy": {
                "@id": "adex:"
            }
        },
        {
            "@id": "adex:isRelatedTo",
            "@type": [
                "adex:TextProperty"
            ],
            "rdfs:comment": "Value associated with RelationshipValue class. Contains IRI(s) that specify the relationship object(s).",
            "rdfs:label": "isRelatedTo",
            "adex:domainIncludes": [
                {
                    "@id": "adex:RelationshipValue"
                }
            ],
            "adex:rangeIncludes": [
                {
                    "@id": "adex:Text",
                    "@type": "@id"
                },
                {
                    "@id": "adex:Text",
                    "@type": "@id",
                    "@container": "@set"
                },
                {
                    "@id": "adex:ValueDescriptor"
                }
            ]
        },
        {
            "@id": "adex:dataSampleFile",
            "@type": [
                "adex:Relationship"
            ],
            "rdfs:comment": "Sample file download link for the resource",
            "rdfs:label": "dataSampleFile",
            "adex:domainIncludes": [
                {
                    "@id": "adex:ResourceGroup"
                },
                {
                    "@id": "adex:Resource"
                }
            ],
            "adex:rangeIncludes": [
                {
                    "@container": "@list",
                    "@id": "adex:Text"
                },
                {
                    "@container": "@list",
                    "@id": "adex:RelationshipValue"
                }
            ],
            "rdfs:isDefinedBy": {
                "@id": "adex:"
            }
        },
        {
            "@id": "adex:secureDataFields",
            "@type": [
                "adex:TextProperty"
            ],
            "rdfs:comment": "List of properties/fields/attributes contained in the data available from the resources associated with a given resource Group which are secure, i.e., need authorization from the auth server to access these fields for a given resource.",
            "rdfs:label": "secureDataFields",
            "adex:domainIncludes": [
                {
                    "@id": "adex:DataFieldListValue"
                }
            ],
            "adex:rangeIncludes": [
                {
                    "@id": "adex:Text",
                    "@container": "@set"
                }
            ]
        },
        {
            "@id": "adex:authControlLevel",
            "@type": [
                "adex:TextProperty"
            ],
            "rdfs:comment": "Authorizataion Control Level for resouces associated with a given resource-group.  Individual authorization control level indicates that access control is available per resource, i.e., authorization can be granted/not-granted on a per resource basis for the resources. Group authorization control level indicates that the authorization is available on group level only, i.e., authorization will be granted/not-granted for all the resources associated with the given resource group. ENUM: [GROUP, INDIVIDUAL]. Default value is set to GROUP. This field is applicable only for non-open data, i.e., when the accessPolicy field is set to value other than OPEN.",
            "rdfs:label": "authControlLevel",
            "adex:domainIncludes": [
                {
                    "@id": "adex:ResourceGroup"
                }
            ],
            "adex:rangeIncludes": [
                {
                    "@id": "adex:Text"
                }
            ],
            "rdfs:isDefinedBy": {
                "@id": "adex:"
            }
        },
        {
            "@id": "adex:accessPolicy",
            "@type": [
                "adex:TextProperty"
            ],
            "rdfs:comment": "Defines the access policy for resources belonging to ResourceGroup or an individual Resource. In case of ResourceGroup item, it can take values: [OPEN, SECURE, MIXED]. OPEN implies all Resources in the group are open (and need no authorization token for data access). SECURE implies that all Resources are secured and will need authorization token for access. MIXED implies that some of Resource items may be open. In case of accessPolicy being set to MIXED in the resource group, the individual resource items will further qualify the access policy using this field. In case of Resource item, it will take values from: [OPEN, SECURE].",
            "rdfs:label": "accessPolicy",
            "adex:domainIncludes": [
                {
                    "@id": "adex:ResourceGroup"
                },
                {
                    "@id": "adex:Resource"
                }
            ],
            "adex:rangeIncludes": [
                {
                    "@id": "adex:Text"
                }
            ],
            "rdfs:isDefinedBy": {
                "@id": "adex:"
            }
        },
        {
            "@id": "adex:landmark",
            "@type": [
                "adex:GeoProperty"
            ],
            "rdfs:comment": "A physical distinguishing feature on land that marks a locality or a place.",
            "rdfs:label": "landmark",
            "adex:domainIncludes": [],
            "adex:rangeIncludes": [
                {
                    "@id": "adex:Text"
                },
                {
                    "@id": "adex:ValueDescriptor"
                }
            ],
            "rdfs:isDefinedBy": {
                "@id": "adex:"
            }
        },
        {
            "@id": "adex:itemStatus",
            "@type": [
                "adex:TextProperty"
            ],
            "rdfs:comment": "Status of a catalouge item. ENUM: [ACTIVE, DEPRECATED].",
            "rdfs:label": "itemStatus",
            "adex:domainIncludes": [
                {
                    "@id": "adex:ADEXEntity"
                }
            ],
            "adex:rangeIncludes": [
                {
                    "@id": "adex:Text"
                }
            ],
            "rdfs:isDefinedBy": {
                "@id": "adex:"
            }
        },
        {
            "@id": "adex:dataSchema",
            "@type": [
                "adex:TextProperty"
            ],
            "rdfs:comment": "Associated data schema. Specified as an URI (linking it to one of the known data type vocabulary, e.g., xsd)",
            "rdfs:label": "dataSchema",
            "adex:domainIncludes": [
                {
                    "@id": "adex:ValueDescriptor"
                }
            ],
            "adex:rangeIncludes": [
                {
                    "@id": "adex:Text",
                    "@type": "@id"
                }
            ],
            "rdfs:isDefinedBy": {
                "@id": "adex:"
            }
        },
        {
            "@id": "adex:dataSample",
            "@type": [
                "adex:TextProperty"
            ],
            "rdfs:comment": "Stringified sample object of the resource",
            "rdfs:label": "dataSample",
            "adex:domainIncludes": [
                {
                    "@id": "adex:ResourceGroup"
                },
                {
                    "@id": "adex:Resource"
                }
            ],
            "adex:rangeIncludes": [
                {
                    "@id": "adex:Text"
                }
            ],
            "rdfs:isDefinedBy": {
                "@id": "adex:"
            }
        },
        {
            "@id": "adex:hasObject",
            "@type": [
                "adex:TextProperty"
            ],
            "rdfs:comment": "Value associated with RelationshipValue class. Contains IRI(s) that specify the relationship object(s).",
            "rdfs:label": "hasObject",
            "adex:domainIncludes": [
                {
                    "@id": "adex:RelationshipValue"
                }
            ],
            "adex:rangeIncludes": [
                {
                    "@id": "adex:Text",
                    "@type": "@id"
                },
                {
                    "@id": "adex:Text",
                    "@type": "@id",
                    "@container": "@set"
                },
                {
                    "@id": "adex:ValueDescriptor"
                }
            ]
        },
        {
            "@id": "adex:longitude",
            "@type": [
                "adex:GeoProperty"
            ],
            "rdfs:comment": "Longitude of a place. Specified in WGS 84 CRS (https://en.wikipedia.org/wiki/World_Geodetic_System)",
            "rdfs:label": "longitude",
            "adex:domainIncludes": [
                {
                    "@id": "adex:GeoCoordinates"
                },
                {
                    "@id": "adex:Place"
                }
            ],
            "adex:rangeIncludes": [
                {
                    "@id": "adex:Number"
                },
                {
                    "@id": "adex:Text"
                }
            ],
            "skos:exactMatch": {
                "@id": "schema:longitude"
            },
            "rdfs:isDefinedBy": {
                "@id": "adex:"
            }
        },
        {
            "@id": "adex:areaServed",
            "@type": [
                "adex:GeoProperty"
            ],
            "rdfs:comment": "Area served by the entity or a service.",
            "rdfs:label": "areaServed",
            "rdfs:isDefinedBy": {
                "@id": "adex:"
            },
            "adex:domainIncludes": [
                {
                    "@id": "adex:ModelInfo"
                }
            ],
            "adex:rangeIncludes": [
                {
                    "@id": "adex:Text"
                }
            ]
        },
        {
            "@id": "adex:id",
            "@type": [
                "adex:TextProperty"
            ],
            "rdfs:comment": "ID of the entity.",
            "rdfs:label": "id",
            "adex:domainIncludes": [
                {
                    "@id": "adex:ADEXEntity"
                }
            ],
            "adex:rangeIncludes": [
                {
                    "@id": "adex:Text"
                }
            ],
            "rdfs:isDefinedBy": {
                "@id": "adex:"
            }
        },
        {
            "@id": "adex:accessObjectType",
            "@type": [
                "adex:TextProperty"
            ],
            "rdfs:comment": "Type of access object. ENUM: [OpenAPI, AsyncAPI]",
            "rdfs:label": "accessObjectType",
            "adex:domainIncludes": [
                {
                    "@id": "adex:AccessObjectInfoValue"
                }
            ],
            "adex:rangeIncludes": [
                {
                    "@id": "adex:Text"
                }
            ]
        },
        {
            "@id": "adex:authType",
            "@type": [
                "adex:TextProperty"
            ],
            "rdfs:comment": "Identification of the auth scheme used for a given resource.  ENUM: [ADEXAUTH].",
            "rdfs:label": "authType",
            "adex:domainIncludes": [
                {
                    "@id": "adex:AuthServerInfoValue"
                }
            ],
            "adex:rangeIncludes": [
                {
                    "@id": "adex:Text"
                }
            ]
        },
        {
            "@id": "adex:unitCode",
            "@type": [
                "adex:TextProperty"
            ],
            "rdfs:comment": "The unit of measurement given using the UN/CEFACT Common Code (3 characters) or a URL. Other codes/unit vocabularies may be used with a prefix",
            "rdfs:label": "unitCode",
            "adex:domainIncludes": [
                {
                    "@id": "adex:ValueDescriptor"
                }
            ],
            "adex:rangeIncludes": [
                {
                    "@id": "adex:Text"
                },
                {
                    "@id": "adex:Text",
                    "@type": "@id"
                }
            ],
            "skos:exactMatch": {
                "@id": "schema:unitCode"
            },
            "rdfs:isDefinedBy": {
                "@id": "adex:"
            }
        },
        {
            "@id": "adex:adexResourceAPIs",
            "@type": [
                "adex:TextProperty"
            ],
            "rdfs:comment": "The set of ADEX resource APIs supported by a given ResourceGroup. ENUM: [TEMPORAL, SPATIAL, ATTR, TEXT]",
            "rdfs:label": "adexResourceAPIs",
            "adex:domainIncludes": [
                {
                    "@id": "adex:ResourceGroup",
                    "adex:requiredProperty": true
                },
                {
                    "@id": "adex:Resource"
                }
            ],
            "adex:rangeIncludes": [
                {
                    "@id": "adex:Text",
                    "@container": "@set"
                }
            ],
            "rdfs:isDefinedBy": {
                "@id": "adex:"
            }
        },
        {
            "@id": "adex:modelURL",
            "@type": [
                "adex:TextProperty"
            ],
            "rdfs:comment": "URL providing further information of a specific model associated with an entity, e.g., sensor, device etc.",
            "rdfs:label": "modelURL",
            "rdfs:isDefinedBy": {
                "@id": "adex:"
            },
            "adex:domainIncludes": [
                {
                    "@id": "adex:ModelInfo"
                }
            ],
            "adex:rangeIncludes": [
                {
                    "@id": "adex:Text"
                }
            ]
        },
        {
            "@id": "adex:relatedEntity",
            "@type": [
                "adex:Relationship"
            ],
            "rdfs:comment": "ID of the associated entity.",
            "rdfs:label": "relatedEntity",
            "adex:domainIncludes": [
                {
                    "@id": "adex:ADEXEntity"
                }
            ],
            "adex:rangeIncludes": [
                {
                    "@id": "adex:Text"
                },
                {
                    "@id": "adex:RelationshipValue"
                }
            ],
            "rdfs:isDefinedBy": {
                "@id": "adex:"
            }
        },
        {
            "@id": "adex:location",
            "@type": [
                "adex:GeoProperty"
            ],
            "rdfs:comment": "Location associated with a resource Item (a spatial point), a group of resource items (a spatial region) or even an observation in case of a mobile sensor.",
            "rdfs:label": "location",
            "adex:domainIncludes": [
                {
                    "@id": "adex:Resource"
                },
                {
                    "@id": "adex:ResourceGroup"
                },
                {
                    "@id": "adex:Provider"
                },
                {
                    "@id": "adex:ResourceServer"
                },
                {
                    "@id": "adex:Organization"
                }
            ],
            "adex:rangeIncludes": [
                {
                    "@id": "adex:Point"
                },
                {
                    "@id": "adex:GeoJSONGeometry"
                },
                {
                    "@id": "adex:Place"
                },
                {
                    "@id": "adex:Text"
                },
                {
                    "@id": "adex:ValueDescriptor"
                }
            ],
            "rdfs:isDefinedBy": {
                "@id": "adex:"
            },
            "skos:exactMatch": {
                "@id": "schema:location"
            }
        },
        {
            "@id": "adex:repositoryURL",
            "@type": [
                "adex:Relationship"
            ],
            "rdfs:comment": "A URL pointing to a repository containing additional resources or code pertaining to this entity.",
            "rdfs:label": "repositoryURL",
            "rdfs:isDefinedBy": {
                "@id": "adex:"
            },
            "adex:domainIncludes": [],
            "adex:rangeIncludes": [
                {
                    "@id": "adex:Text",
                    "@type": "@id"
                },
                {
                    "@id": "adex:RelationshipValue"
                }
            ]
        },
        {
            "@id": "adex:name",
            "@type": [
                "adex:TextProperty"
            ],
            "rdfs:comment": "Name of the entity.",
            "rdfs:label": "name",
            "adex:domainIncludes": [
                {
                    "@id": "adex:Place"
                },
                {
                    "@id": "adex:Organization"
                },
                {
                    "@id": "adex:RelationshipValue"
                },
                {
                    "@id": "adex:ADEXEntity",
                    "adex:requiredProperty": true
                }
            ],
            "adex:rangeIncludes": [
                {
                    "@id": "adex:Text"
                },
                {
                    "@id": "adex:ValueDescriptor"
                }
            ],
            "skos:exactMatch": {
                "@id": "schema:name"
            },
            "rdfs:isDefinedBy": {
                "@id": "adex:"
            }
        },
        {
            "@id": "adex:resourceServer",
            "@type": [
                "adex:Relationship"
            ],
            "rdfs:comment": "IRI pointing to the ResourceServer entity for a given Resource or ResourceGroup.",
            "rdfs:label": "resourceServer",
            "adex:domainIncludes": [
                {
                    "@id": "adex:Resource"
                },
                {
                    "@id": "adex:ResourceGroup"
                }
            ],
            "adex:rangeIncludes": [
                {
                    "@id": "adex:Text",
                    "@type": "@id"
                },
                {
                    "@id": "adex:RelationshipValue"
                }
            ]
        },
        {
            "@id": "adex:dataDescriptorLabel",
            "@type": [
                "adex:TextProperty"
            ],
            "rdfs:comment": "Human readable label for an entity",
            "rdfs:label": "dataDescriptorLabel",
            "adex:domainIncludes": [
                {
                    "@id": "adex:DataDescriptor"
                }
            ],
            "adex:rangeIncludes": [
                {
                    "@id": "adex:Text"
                }
            ],
            "rdfs:isDefinedBy": {
                "@id": "adex:"
            }
        },
        {
            "@id": "adex:authServerURL",
            "@type": [
                "adex:Relationship"
            ],
            "rdfs:comment": "URL of the ADEX authorization server used for a given resource.",
            "rdfs:label": "authServerURL",
            "adex:domainIncludes": [
                {
                    "@id": "adex:AuthServerInfoValue"
                }
            ],
            "adex:rangeIncludes": [
                {
                    "@id": "adex:Text",
                    "@type": "@id"
                },
                {
                    "@id": "adex:RelationshipValue"
                }
            ]
        },
        {
            "@id": "adex:brandName",
            "@type": [
                "adex:TextProperty"
            ],
            "rdfs:comment": "Name of the brand associated with an entity, e.g., sensor, device etc.",
            "rdfs:label": "brandName",
            "rdfs:isDefinedBy": {
                "@id": "adex:"
            },
            "adex:domainIncludes": [
                {
                    "@id": "adex:ModelInfo"
                }
            ],
            "adex:rangeIncludes": [
                {
                    "@id": "adex:Text"
                }
            ],
            "skos:exactMatch": {
                "@id": "Fiware:brandName"
            }
        },
        {
            "@id": "adex:resourceServerStreamingAccessURL",
            "@type": [
                "adex:Relationship"
            ],
            "rdfs:comment": "Resource Server URL for data access based on Streaming",
            "rdfs:label": "resourceServerStreamingAccessURL",
            "adex:domainIncludes": [
                {
                    "@id": "adex:ResourceServer"
                }
            ],
            "adex:rangeIncludes": [
                {
                    "@id": "adex:Text",
                    "@type": "@id"
                }
            ]
        },
        {
            "@id": "adex:value",
            "@type": [
                "rdf:Property"
            ],
            "rdfs:comment": "Value of the quantity being described in the ValueDescriptor object.",
            "rdfs:label": "value",
            "adex:domainIncludes": [
                {
                    "@id": "adex:ValueDescriptor"
                }
            ],
            "adex:rangeIncludes": [
                {
                    "@id": "adex:Number"
                },
                {
                    "@id": "adex:Text"
                },
                {
                    "@id": "adex:Boolean"
                },
                {
                    "@id": "adex:NumericArray"
                },
                {
                    "@id": "adex:StructuredValue"
                }
            ],
            "rdfs:isDefinedBy": {
                "@id": "adex:"
            }
        },
        {
            "@id": "adex:openDataFields",
            "@type": [
                "adex:TextProperty"
            ],
            "rdfs:comment": "List of properties/fields/attributes contained in the data available from the resources associated with a given resource Group which are open, i.e., no authorization is required to access these fields for a given resource.",
            "rdfs:label": "openDataFields",
            "adex:domainIncludes": [
                {
                    "@id": "adex:DataFieldListValue"
                }
            ],
            "adex:rangeIncludes": [
                {
                    "@id": "adex:Text",
                    "@container": "@set"
                }
            ]
        },
        {
            "@id": "adex:latitude",
            "@type": [
                "adex:GeoProperty"
            ],
            "rdfs:comment": "Latitude of a place. Specified in WGS 84 CRS (https://en.wikipedia.org/wiki/World_Geodetic_System)",
            "rdfs:label": "latitude",
            "adex:domainIncludes": [
                {
                    "@id": "adex:GeoCoordinates"
                },
                {
                    "@id": "adex:Place"
                }
            ],
            "adex:rangeIncludes": [
                {
                    "@id": "adex:Number"
                },
                {
                    "@id": "adex:Text"
                }
            ],
            "skos:exactMatch": {
                "@id": "schema:latitude"
            },
            "rdfs:isDefinedBy": {
                "@id": "adex:"
            }
        },
        {
            "@id": "adex:mediaURL",
            "@type": [
                "adex:TextProperty"
            ],
            "rdfs:comment": "URL providing further information of any image(s) or media of the complaint or place.",
            "rdfs:label": "mediaURL",
            "adex:domainIncludes": [],
            "adex:rangeIncludes": [
                {
                    "@container": "@list",
                    "@id": "adex:Text"
                },
                {
                    "@id": "adex:ValueDescriptor"
                }
            ],
            "rdfs:isDefinedBy": {
                "@id": "adex:"
            },
            "skos:exactMatch": {
                "@id": "open311:media_url"
            }
        },
        {
            "@id": "adex:modelName",
            "@type": [
                "adex:TextProperty"
            ],
            "rdfs:comment": "Name of a specific model associated with an entity, e.g., sensor, device etc.",
            "rdfs:label": "modelName",
            "rdfs:isDefinedBy": {
                "@id": "adex:"
            },
            "adex:domainIncludes": [
                {
                    "@id": "adex:ModelInfo"
                }
            ],
            "adex:rangeIncludes": [
                {
                    "@id": "adex:Text"
                }
            ],
            "skos:exactMatch": {
                "@id": "Fiware:modelName"
            }
        },
        {
            "@id": "adex:resourceType",
            "@type": [
                "adex:TextProperty"
            ],
            "rdfs:comment": "Type of resource. ENUM: [MESSAGESTREAM, DATASET, FILE, GSLAYER, MEDIASTREAM].",
            "rdfs:label": "resourceType",
            "adex:domainIncludes": [
                {
                    "@id": "adex:ResourceGroup",
                    "adex:requiredProperty": true
                },
                {
                    "@id": "adex:Resource"
                }
            ],
            "adex:rangeIncludes": [
                {
                    "@id": "adex:Text"
                }
            ],
            "rdfs:isDefinedBy": {
                "@id": "adex:"
            }
        },
        {
            "@id": "adex:label",
            "@type": [
                "adex:TextProperty"
            ],
            "rdfs:comment": "Human readable label for an entity",
            "rdfs:label": "label",
            "adex:domainIncludes": [
                {
                    "@id": "adex:ADEXEntity"
                }
            ],
            "adex:rangeIncludes": [
                {
                    "@id": "adex:Text"
                }
            ],
            "rdfs:isDefinedBy": {
                "@id": "adex:"
            }
        },
        {
            "@id": "adex:dataDescriptorName",
            "@type": [
                "adex:TextProperty"
            ],
            "rdfs:comment": "Name of the entity.",
            "rdfs:label": "dataDescriptorName",
            "adex:domainIncludes": [
                {
                    "@id": "adex:DataDescriptor"
                }
            ],
            "adex:rangeIncludes": [
                {
                    "@id": "adex:Text"
                }
            ],
            "skos:exactMatch": {
                "@id": "schema:name"
            },
            "rdfs:isDefinedBy": {
                "@id": "adex:"
            }
        },
        {
            "@id": "adex:measAccuracy",
            "@type": [
                "adex:QuantitativeProperty"
            ],
            "rdfs:comment": "Accuracy of a measurement. Maximum difference that can exist between the actual value and the measured value. It can be specified in relative as well as absolute terms.",
            "rdfs:label": "measAccuracy",
            "adex:domainIncludes": [
                {
                    "@id": "adex:ValueDescriptor"
                }
            ],
            "adex:rangeIncludes": [
                {
                    "@id": "adex:Text"
                },
                {
                    "@id": "adex:ValueDescriptor"
                }
            ],
            "rdfs:isDefinedBy": {
                "@id": "adex:"
            }
        },
        {
            "@id": "adex:aqiMajorPollutant",
            "@type": [
                "adex:TextProperty"
            ],
            "rdfs:comment": "Major pollutant in the Air Quality Index (AQI).",
            "rdfs:label": "aqiMajorPollutant",
            "rdfs:isDefinedBy": {
                "@id": "adex:"
            },
            "adex:domainIncludes": [
                {
                    "@id": "adex:Weather"
                }
            ],
            "adex:rangeIncludes": [
                {
                    "@id": "adex:Text"
                },
                {
                    "@id": "adex:ValueDescriptor"
                }
            ],
            "skos:exactMatch": {
                "@id": "iudx:aqiMajorPollutant"
            }
        },
        {
            "@id": "adex:aqiMajorPollutantForecast",
            "@type": [
                "adex:TextProperty"
            ],
            "rdfs:comment": "Forecasted major air pollutant in the Air Quality Index (AQI) over a certain duration in future.",
            "rdfs:label": "aqiMajorPollutantForecast",
            "rdfs:isDefinedBy": {
                "@id": "adex:"
            },
            "adex:domainIncludes": [
                {
                    "@id": "adex:Weather"
                }
            ],
            "adex:rangeIncludes": [
                {
                    "@id": "adex:Text"
                },
                {
                    "@id": "adex:ValueDescriptor"
                }
            ],
            "skos:exactMatch": {
                "@id": "iudx:aqiMajorPollutantForecast"
            }
        },
        {
            "@id": "adex:weatherType",
            "@type": [
                "adex:TextProperty"
            ],
            "rdfs:comment": "Observed weather type or status. Represented by a comma separated list of weather types, e.g., cloudy, sunny etc.",
            "rdfs:label": "weatherType",
            "rdfs:isDefinedBy": {
                "@id": "adex:"
            },
            "adex:domainIncludes": [
                {
                    "@id": "adex:Weather"
                }
            ],
            "adex:rangeIncludes": [
                {
                    "@id": "adex:Text"
                },
                {
                    "@id": "adex:ValueDescriptor"
                }
            ],
            "skos:exactMatch": {
                "@id": "Fiware:weatherType"
            }
        }
    ],
    "@context": {
        "iudx": "https://voc.iudx.org.in/",
        "owl": "http://www.w3.org/2002/07/owl#",
        "rdf": "http://www.w3.org/1999/02/22-rdf-syntax-ns#",
        "skos": "http://www.w3.org/2004/02/skos/core#",
        "schema": "http://schema.org/",
        "rdfs": "http://www.w3.org/2000/01/rdf-schema#",
        "adex": "https://agrijson.adex.org.in/",
        "geojson": "https://purl.org/geojson/vocab#",
        "xsd": "http://www.w3.org/2001/XMLSchema#",
        "qudt": "http://qudt.org/vocab/unit/"
    }
}